

3.3 Exponential families

Def. A family of pdf or pmf is called an **exponential family** if it has the form

$$f(x|\theta) = c(\theta) h(x) \exp \left\{ \sum_{i=1}^k w_i(\theta) t_i(x) \right\}, x \in \mathcal{X}$$

$$= c(\theta) h(x) \exp \langle w(\theta), t(x) \rangle \quad (*)$$

$$\begin{aligned} &\uparrow \\ w(\theta) &= (w_1(\theta), \dots, w_k(\theta)) \\ t(x) &= (t_1(x), \dots, t_k(x)) \\ &\uparrow \\ &\text{vector of sufficient statistics} \end{aligned}$$

Here

$$h(x) \geq 0$$

$$t(x) = (t_1(x), \dots, t_k(x))$$

$$w(\theta) = (w_1(\theta), \dots, w_k(\theta))$$

depends on x only

depends on θ only

data

parameter

Clearly, $c(\theta)$ is the reciprocal of the normalizing const

$$1/c(\theta) = \int_{\mathcal{X}} h(x) e^{\langle w(\theta), t(x) \rangle} dx$$

or sum, if \mathcal{X} is discrete

$c(\theta)$ depends only on θ (not x).

Example 1 (Binomial) Let $X \sim \text{Binomial}(n, p)$

$$\begin{aligned}
 f_X(x) &= \binom{n}{x} p^x (1-p)^{n-x}, \quad x = 0, 1, \dots, n \\
 &= (1-p)^n \binom{n}{x} (p/(1-p))^x \\
 &= \underbrace{(1-p)^n}_{c(\theta)} \underbrace{\binom{n}{x}}_{h(x)} \exp \left\{ \underbrace{x}_{t(x)} \log \underbrace{\frac{p}{1-p}}_{w_1(\theta)} \right\} \quad k=1
 \end{aligned}$$

Example 2 (Normal) Let $X \sim N(\mu, \sigma^2)$

$$\begin{aligned}
 f_X(x) &= \frac{1}{\sqrt{2\pi\sigma^2}} \exp -\frac{1}{2\sigma^2} (x-\mu)^2, \quad x \in \mathbb{R} \\
 &\quad \theta = (\mu, \sigma) \in \mathbb{R} \times \mathbb{R}_+ \\
 &= \frac{1}{\sqrt{2\pi\sigma^2}} \exp -\frac{1}{2\sigma^2} (x^2 - 2x\mu + \mu^2) \\
 &= \underbrace{\frac{1}{\sqrt{2\pi\sigma^2}} e^{-\frac{\mu^2}{2\sigma^2}}}_{c(\theta)} \exp \left\{ \underbrace{-\frac{1}{2\sigma^2}}_{w_1(\theta)} \underbrace{x^2}_{t_1(x)} + \underbrace{\frac{\mu}{\sigma^2}}_{w_2(\theta)} \underbrace{x}_{t_2(x)} \right\}
 \end{aligned}$$

Other examples : Poisson, Geometric, Negative binomial, ...
Gamma, Exponential, Log-normal,

Not in the exponential families :

Cauchy
Mixtures

Theorem if X is a Random variable with pdf/pmf in the exponential family of the form (*)

then

$$(1) \quad E \sum_{i=1}^k \frac{\partial w_i(\theta)}{\partial \theta_j} t_i(X) = \frac{\partial}{\partial \theta_j} \log(1/c(\theta)), \text{ for } j=1, \dots, k$$

$$(2) \quad \text{var} \left(\sum_{i=1}^k \frac{\partial w_i(\theta)}{\partial \theta_j} t_i(X) \right) = \frac{\partial^2}{\partial \theta_j^2} \log(1/c(\theta)) - E \left(\sum_{i=1}^k \frac{\partial^2 w_i(\theta)}{\partial \theta_j^2} t_i(X) \right).$$

High-level statement : differentiating the logarithm of the normalizing constant with respect to a parameter results in suitable expectations of suff. statistics

Let's look at a simplified statement

$$w(\theta) = \theta = (\theta_1, \theta_2, \dots, \theta_k) \in \mathbb{R}^k$$

$$t(x) = (t_1(x), t_2(x), \dots, t_k(x)) \in \mathbb{R}^k$$

$$\text{Then } f(x|\theta) = c(\theta) h(x) \exp \langle \theta, t(x) \rangle$$

(1) gives: $E t_j(x) = \frac{\partial}{\partial \theta_j} \log(1/c(\theta))$

(2) gives: $\text{var } t_j(x) = \frac{\partial^2}{\partial \theta_j^2} \log(1/c(\theta))$

Proof of theorem is a simple exercise of calculus.

Example (Binomial)

$$f(x|p) = \underbrace{(1-p)^n}_{c(\theta)} \underbrace{\binom{n}{x}}_{h(x)} \exp \left\{ \underbrace{x}_{t_1(x)} \log \underbrace{\frac{p}{1-p}}_{w_1(\theta)} \right\} \quad k=1$$

$$c(\theta) = (1-p)^n$$

$$\theta \equiv p$$

$$\begin{aligned}\frac{\partial}{\partial \theta} \log(1/c(\theta)) &= -\frac{\partial}{\partial p} n \log(1-p) \\ &= \frac{n}{1-p}.\end{aligned}$$

$$\begin{aligned}\frac{\partial}{\partial \theta} w_1(\theta) &= \frac{\partial}{\partial p} (\log p - \log(1-p)) \\ &= \frac{1}{p} + \frac{1}{1-p} = \frac{1}{p(1-p)}\end{aligned}$$

Applying the theorem

$$\frac{\partial}{\partial \theta} \log(1/c(\theta)) = \mathbb{E} \underbrace{\frac{\partial}{\partial \theta} w_1(\theta)} \underbrace{t_1(X)}$$

$$\frac{n}{1-p} = \mathbb{E} \frac{1}{p(1-p)} X$$

$$n = \mathbb{E} \frac{X}{p}$$

$$\Rightarrow \mathbb{E} X = np.$$

Example (Normal)

$$f_X(x) = \frac{1}{\sqrt{2\pi}\sigma} e^{-\frac{x^2}{2\sigma^2}} \exp \left\{ -\frac{1}{2\sigma^2} x^2 + \frac{\mu}{\sigma^2} x \right\}$$

$$f_X(x) = \underbrace{\frac{1}{\sqrt{2\pi\sigma^2}}}_{c(\theta)} e^{-\frac{\mu^2}{2\sigma^2}} \exp \left\{ \underbrace{-\frac{1}{2\sigma^2}}_{w_1(\theta)} \underbrace{x^2}_{t_1(x)} + \underbrace{\frac{\mu}{\sigma^2}}_{w_2(\theta)} \underbrace{x}_{t_2(x)} \right\}$$

$$w(\theta) = \left(-\frac{1}{2\sigma^2}, \frac{\mu}{\sigma^2} \right)$$

$$\begin{aligned} \frac{\partial}{\partial \mu} \log(1/c(\theta)) &= \frac{\partial}{\partial \mu} \left(\log(\sqrt{2\pi\sigma^2}) + \frac{\mu^2}{2\sigma^2} \right) \\ &= \frac{\mu}{\sigma^2} \end{aligned}$$

$$\frac{\partial}{\partial \mu} w_2(\theta) = \frac{\partial}{\partial \mu} \left(\frac{\mu}{\sigma^2} \right) = \frac{1}{\sigma^2}$$

Applying the theorem

$$\begin{aligned} \frac{\partial}{\partial \mu} \log(1/c(\theta)) &= \mathbb{E} \left(\underbrace{\frac{\partial}{\partial \mu} w_2(\theta)}_{\frac{1}{\sigma^2}} t_2(x) + \underbrace{\left(\frac{\partial}{\partial \mu} w_1(\theta) \right) t_1(x)}_0 \right) \\ \frac{\mu}{\sigma^2} &= \frac{1}{\sigma^2} \mathbb{E} X \end{aligned}$$

$$\text{So } \mathbb{E} X = \mu$$

To obtain $\mathbb{E} t_2(x) = \mathbb{E} X^2$:

To obtain $E t_2(X) = EX^2$:

$$\begin{aligned}\frac{\partial}{\partial \sigma} \log\left(\frac{1}{c(\theta)}\right) &= \frac{\partial}{\partial \sigma} \left(\log \sqrt{2\pi\sigma^2} + \frac{\mu^2}{2\sigma^2} \right) \\ &= \frac{1}{\sigma} - \mu^2 \frac{1}{\sigma^3}\end{aligned}$$

$$\frac{\partial}{\partial \sigma} w_1(\theta) = \frac{\partial}{\partial \sigma} \left(-\frac{1}{2\sigma^2} \right) = \frac{1}{\sigma^3}$$

$$\frac{\partial}{\partial \sigma} w_2(\theta) = \frac{\partial}{\partial \sigma} \left(\frac{\mu}{\sigma^2} \right) = -2\mu \frac{1}{\sigma^3}$$

Applying the theorem

$$\frac{\partial}{\partial \sigma} \log\left(\frac{1}{c(\theta)}\right) = E\left(\frac{\partial}{\partial \sigma} w_1(\theta)\right) t_1(X) + \left(\frac{\partial}{\partial \sigma} w_2(\theta)\right) t_2(X)$$

$$\frac{1}{\sigma} - \mu^2 \frac{1}{\sigma^3} = \frac{1}{\sigma^3} EX^2 - \frac{2\mu}{\sigma^3} EX$$

$$\sigma^2 - \mu^2 = EX^2 - 2\mu^2$$

$$\begin{aligned}\text{Hence } EX^2 &= \sigma^2 + \mu^2 \\ \Rightarrow \text{var } X &= EX^2 - (EX)^2 \\ &= EX^2 - \mu^2 \\ &= \sigma^2.\end{aligned}$$